<?xml version="1.0" encoding="UTF-8"?>
<section xml:id="CFL-intro" xmlns:xi="http://www.w3.org/2001/XInclude">
  <title>Recursive inference, trees, and derivations</title>
  <objectives>
    <ol>
      <li>Learn stuff</li>
    </ol>
  </objectives>
  <p>
    In class, we looked at the following example grammar and tried to write down
    a recursive inference table for the sentence
    <m>(((P \vee Q) \wedge R) \vee (Q \wedge (\neg P)))</m>.
    <md>
      <mrow>E \amp \to (EBE) \mid (UE) \mid C \mid V</mrow>
      <mrow>B \amp \to \wedge \mid \vee \mid \; \to \; \mid \; \leftrightarrow</mrow>
      <mrow>U \amp \to \neg</mrow>
      <mrow>C \amp \to \bot \mid \top</mrow>
      <mrow>V \amp \to P \mid Q \mid R</mrow>
    </md>
    The table below shows one solution.
  </p>
  <table xml:id="table-recursive-inference-kozen">
    <title>Recursive inference for <m>(((P \vee Q) \wedge R) \vee (Q \wedge (\neg P)))</m></title>
    <tabular>
      <row header="yes" bottom="medium">
        <cell></cell>
        <cell>String</cell>
        <cell>Variable</cell>
        <cell>Production</cell>
        <cell>Strings used</cell>
      </row>
      <row>
        <cell>1</cell>
        <cell><m>P</m></cell>
        <cell><m>V</m></cell>
        <cell><m>V \to P</m></cell>
        <cell><mdash/></cell>
      </row>
      <row>
        <cell>2</cell>
        <cell><m>Q</m></cell>
        <cell><m>V</m></cell>
        <cell><m>V \to Q</m></cell>
        <cell><mdash/></cell>
      </row>
      <row>
        <cell>3</cell>
        <cell><m>V</m></cell>
        <cell><m>E</m></cell>
        <cell><m>E \to V</m></cell>
        <cell><mdash/></cell>
      </row>
      <row>
        <cell>4</cell>
        <cell><m>P</m></cell>
        <cell><m>E</m></cell>
        <cell><m>E \to V</m></cell>
        <cell>1</cell>
      </row>
      <row>
        <cell>5</cell>
        <cell><m>Q</m></cell>
        <cell><m>E</m></cell>
        <cell><m>E \to V</m></cell>
        <cell>2</cell>
      </row>
      <row>
        <cell>6</cell>
        <cell><m>\vee</m></cell>
        <cell><m>B</m></cell>
        <cell><m>B \to \vee</m></cell>
        <cell><mdash/></cell>
      </row>
      <row>
        <cell>7</cell>
        <cell><m>(P \vee Q)</m></cell>
        <cell><m>E</m></cell>
        <cell><m>E \to (EBE)</m></cell>
        <cell>4, 5, 6</cell>
      </row>
      <row>
        <cell>8</cell>
        <cell><m>R</m></cell>
        <cell><m>V</m></cell>
        <cell><m>V \to R</m></cell>
        <cell><mdash/></cell>
      </row>
      <row>
        <cell>9</cell>
        <cell><m>R</m></cell>
        <cell><m>E</m></cell>
        <cell><m>E \to V</m></cell>
        <cell>8</cell>
      </row>
      <row>
        <cell>10</cell>
        <cell><m>\wedge</m></cell>
        <cell><m>B</m></cell>
        <cell><m>B \to \wedge</m></cell>
        <cell><mdash/></cell>
      </row>
      <row>
        <cell>11</cell>
        <cell><m>((P \vee Q) \wedge R)</m></cell>
        <cell><m>E</m></cell>
        <cell><m>E \to (EBE)</m></cell>
        <cell>7, 10, 9</cell>
      </row>
      <row>
        <cell>12</cell>
        <cell><m>\neg</m></cell>
        <cell><m>U</m></cell>
        <cell><m>U \to \neg</m></cell>
        <cell><mdash/></cell>
      </row>
      <row>
        <cell>13</cell>
        <cell><m>(\neg P)</m></cell>
        <cell><m>E</m></cell>
        <cell><m>E \to (UE)</m></cell>
        <cell>12, 4</cell>
      </row>
      <row>
        <cell>14</cell>
        <cell><m>(Q \wedge (\neg P))</m></cell>
        <cell><m>E</m></cell>
        <cell><m>E \to (EBE)</m></cell>
        <cell>5, 10, 13</cell>
      </row>
      <row bottom="medium">
        <cell>15</cell>
        <cell><m>(((P \vee Q) \wedge R) \vee (Q \wedge (\neg P)))</m></cell>
        <cell><m>E</m></cell>
        <cell><m>E \to (EBE)</m></cell>
        <cell>6, 14, 11</cell>
      </row>
    </tabular>
  </table>
</section>
